depict a bright future

verif/trie/functional/kv.v
@@ -6,19 +6,185 @@ Module Type KEY_TYPE.
   Parameter type: Type.
 End KEY_TYPE.
 
-Module Type KV_STORE (KeyType: KEY_TYPE).
-  Parameter store: Type -> Type.
+Module Type KV_STORE (KeyType: KEY_TYPE) (ValueType: VALUE_TYPE).
+  Parameter store: Type.
   Definition key: Type := KeyType.type.
-  Variable value: Type.
-  Parameter empty: store value.
-  Parameter get: key -> store value -> option value.
-  Parameter put: key -> value -> store value -> store value.
+  Definition value: Type := ValueType.type.
+  Definition default_val: value := ValueType.default.
+  Definition inhabitant_value: Inhabitant value := ValueType.inhabitant_value.
+  Parameter empty: store.
+  Parameter get: key -> store -> value.
+  Parameter put: key -> value -> store -> store.
   Axiom get_empty: forall k,
-      get k empty = None.
+      get k empty = default_val.
   Axiom get_put_same: forall k v s,
-      get k (put k v s) = Some v.
+      get k (put k v s) = v.
   Axiom get_put_diff: forall k1 k2 v s,
       k1 <> k2 -> get k1 (put k2 v s) = get k1 s.
 End KV_STORE.
 
-(* TODO: An functional implementation of [KV_STORE] *)
+(* Transforming a standard kv-store into a list representation *)
+(* 1. we need to make sure that this module conforms KV_STORE, for convenience of client *)
+(* 2. we need to make sure that the operations commutes *)
+
+Module Type ORD_KEY_TYPE <: KEY_TYPE.
+  Include KEY_TYPE.
+  Parameter le: type -> type -> Prop.
+  Notation "A <= B" := (le A B).
+  Notation "A > B" := (~ (le A B)).
+  Parameter le_dec: forall (x y: type), {x <= y} + {x > y}.
+  Axiom le_antisym: forall (x y: type), x <= y -> y <= x -> x = y.
+  Axiom le_refl: forall (x: type), x <= x.
+  Axiom le_trans: forall (x y z: type), x <= y -> y <= z -> x <= z.
+  Axiom gt_le: forall (x y: type), y > x -> x <= y.
+  Parameter EqDec: EqDec type.
+End ORD_KEY_TYPE.
+
+Module SortedListStore (KeyType: ORD_KEY_TYPE) (ValueType: VALUE_TYPE) <: KV_STORE KeyType ValueType.
+  Definition key: Type := KeyType.type.
+  Definition value: Type := ValueType.type.
+  Definition default_val: value := ValueType.default.
+  Instance inhabitant_value: Inhabitant value := ValueType.inhabitant_value.
+  Instance EqDec_key: EqDec key := KeyType.EqDec.
+  Definition store: Type := list (key * value).
+  Definition empty: store := nil.
+  Fixpoint get (k: key) (s: store) :=
+    match s with
+    | (k', v') :: l' =>
+      if eq_dec k k' then
+        v'
+      else get k l'
+    | nil => default_val
+    end.
+
+  Fixpoint put (k: key) (v: value) (s: store) :=
+    match s with
+    | (k', v') :: l' =>
+      if KeyType.le_dec k k' then
+        if eq_dec k k' then
+          (k, v) :: l'
+        else
+          (k, v) :: (k', v') :: l'
+      else
+        (k', v') :: (put k v l')
+    | nil => (k, v) :: nil
+    end.
+
+  Theorem get_empty: forall k, get k empty = default_val.
+  Proof.
+    intros.
+    reflexivity.
+  Qed.
+
+  Theorem get_put_same: forall k v s,
+      get k (put k v s) = v.
+  Proof.
+    induction s as [ | [k' v'] ?].
+    - simpl.
+      rewrite if_true by auto.
+      reflexivity.
+    - simpl.
+      if_tac; simpl; if_tac; simpl.
+      + rewrite if_true by auto.
+        reflexivity.
+      + rewrite if_true by auto.
+        reflexivity.
+      + subst.
+        exfalso.
+        apply H.
+        apply KeyType.le_refl.
+      + assumption.
+  Qed.
+
+  Theorem get_put_diff: forall k1 k2 v s,
+      k1 <> k2 -> get k1 (put k2 v s) = get k1 s.
+  Proof.
+    induction s as [ | [k' v'] ?]; intros.
+    - simpl.
+      rewrite if_false by auto.
+      reflexivity.
+    - simpl.
+      if_tac; simpl; if_tac; simpl; subst.
+      + rewrite ?if_false by auto.
+        reflexivity.
+      + rewrite if_false by auto.
+        reflexivity.
+      + reflexivity.
+      + specialize (IHs H).
+        assumption.
+  Qed.
+
+  Import KeyType.
+
+  (* sorted invariant *)
+  Inductive sorted: store -> Prop :=
+  | sorted_nil: sorted nil
+  | sorted_cons: forall k v l,
+      Forall (fun binding => le k (fst binding)) l -> 
+      sorted l ->
+      sorted ((k, v) :: l).
+
+  Hint Constructors sorted.
+
+  Lemma put_sorted_aux (k k': key) (v: value) (s: store):
+    k' > k ->
+    Forall (fun binding => le k (fst binding)) s ->
+    Forall (fun binding => le k (fst binding)) (put k' v s).
+  Proof.
+    induction s as [ | [k'' v''] ?]; intros.
+    - simpl.
+      constructor; [ | constructor].
+      apply gt_le.
+      assumption.
+    - simpl.
+      if_tac; simpl.
+      + if_tac; simpl.
+        * subst.
+          inversion H0; subst; clear H0.
+          constructor; assumption.
+        * constructor; [ | assumption].
+          apply gt_le in H.
+          assumption.
+      + inversion H0; subst; clear H0.
+        specialize (IHs H H5).
+        constructor; assumption.
+  Qed.
+
+  Lemma put_sorted (k: key) (v: value) (s: store):
+    sorted s -> sorted (put k v s).
+  Proof.
+    induction s as [ | [k' v'] ?]; intros.
+    - simpl.
+      auto.
+    - simpl.
+      if_tac; simpl.
+      + if_tac; simpl.
+        * inversion H; subst; clear H.
+          constructor; assumption.
+        * constructor; [ | assumption].
+          inversion H; subst; clear H.
+          apply Forall_forall.
+          rewrite Forall_forall in H4.
+          intros.
+          assert (k' <= fst x). {
+            inversion H.
+            - subst.
+              apply le_refl.
+            - apply H4.
+              assumption.
+          }
+          apply le_trans with k'; assumption.
+      + inversion H; subst; clear H.
+        constructor; [ | auto].
+        apply put_sorted_aux; assumption.
+  Qed.
+
+End SortedListStore.
+
+Module Transform (KeyType: ORD_KEY_TYPE) (ValueType: VALUE_TYPE) (Source: KV_STORE KeyType ValueType).
+  Module SortedStore := SortedListStore KeyType ValueType.
+  Parameter transform: Source.store -> {store: SortedStore.store | SortedStore.sorted store }.
+  Theorem put_permute (k: KeyType.type) (v: ValueType.type) (s: Source.store):
+    proj1_sig (transform (Source.put k v s)) = SortedStore.put k v(proj1_sig (transform s)). 
+  Admitted.
+End Transform.
