verif/trie/functional/trie.v
@@ -1,0 +1,34 @@
+Require Import VST.floyd.functional_base.
+Require Import common.
+
+Require Import DB.functional.kv.
+Require Import DB.functional.keyslice.
+Require Import DB.functional.bordernode.
+
+Import Lists.List.ListNotations.
+
+Module TrieKey: KEY_TYPE.
+  Definition type: Type := string.
+End TrieKey.
+
+Module Trie.
+  Definition key: Type := TrieKey.type.
+  Variable value: Type.
+
+  Inductive trie: Type :=
+  | trienode_of: list (keyslice * (list link * option string * link)) -> trie
+  with
+  link: Type :=
+  | value_of: value -> link
+  | trie_of: trie -> link
+  | nil: link.
+
+  Module BorderNodeValue: VALUE_TYPE.
+    Definition type := link.
+    Definition default := nil.
+    Definition inhabitant_value := nil.
+  End BorderNodeValue.
+  Module BorderNode := BorderNode BorderNodeValue.
+
+  Definition empty: trie := trienode_of [].
+End Trie.
